examples/sampler/verif_egress_parser.v
@@ -83,7 +83,6 @@ Definition parser_parse_ipv4_spec: func_spec :=
     PATH p
     MOD (Some [["hdr"]]) [["packet_in"]]
     WITH (pin: packet_in) hsample ipv4 result pin'
-         (_: ⊫ᵥ ipv4_repr_val ipv4 \: ipv4_h)
          (_: if is_tcp ipv4 then ⊫ᵥ result \: tcp_h
              else if is_udp ipv4 then ⊫ᵥ result \: udp_h
                   else result = ValBaseNull)
@@ -107,25 +106,25 @@ Proof.
   start_function.
   simpl_format_list.
   step_call (@packet_in_extract_body Info);
-    [ entailer | apply extract_encode; [assumption | reflexivity] |].
-  step_if; change (ValBaseBit _) with (P4BitV 8 IP_PROTOCOLS_TCP) in H1;
-    rewrite abs_ipv4_hdr_eq_eq in H1.
-  - apply is_sval_true_binary_op_eq in H1.
-    change (Val_eqb _ _) with (is_tcp ipv4) in H1. unfold protocol_extract_result.
-    rewrite H1 in *. simpl_format_list.
-    step_call parser_parse_tcp_body; [ entailer | assumption | apply H3 ].
-  - apply is_sval_false_binary_op_eq in H1.
-    change (Val_eqb _ _) with (is_tcp ipv4) in H1.
-    unfold protocol_extract_result. rewrite H1 in *. simpl_format_list.
-    step_if; change (ValBaseBit _) with (P4BitV 8 IP_PROTOCOLS_UDP) in H2;
-      rewrite abs_ipv4_hdr_eq_eq in H2.
-    + apply is_sval_true_binary_op_eq in H2.
-      change (Val_eqb _ _) with (is_udp ipv4) in H2.
-      rewrite H2 in *. simpl_format_list.
-      step_call parser_parse_udp_body; [ entailer | assumption | apply H3 ].
-    + apply is_sval_false_binary_op_eq in H2.
-      change (Val_eqb _ _) with (is_udp ipv4) in H2.
-      rewrite H2 in *. do 4 simpl_format_list. rewrite app_nil_r.
+    [ entailer | apply extract_encode; [ apply ext_val_typ_ipv4 | reflexivity] |].
+  step_if; change (ValBaseBit _) with (P4BitV 8 IP_PROTOCOLS_TCP) in H0;
+    rewrite abs_ipv4_hdr_eq_eq in H0.
+  - apply is_sval_true_binary_op_eq in H0.
+    change (Val_eqb _ _) with (is_tcp ipv4) in H0. unfold protocol_extract_result.
+    rewrite H0 in *. simpl_format_list.
+    step_call parser_parse_tcp_body; [ entailer | assumption | apply H2 ].
+  - apply is_sval_false_binary_op_eq in H0.
+    change (Val_eqb _ _) with (is_tcp ipv4) in H0.
+    unfold protocol_extract_result. rewrite H0 in *. simpl_format_list.
+    step_if; change (ValBaseBit _) with (P4BitV 8 IP_PROTOCOLS_UDP) in H1;
+      rewrite abs_ipv4_hdr_eq_eq in H1.
+    + apply is_sval_true_binary_op_eq in H1.
+      change (Val_eqb _ _) with (is_udp ipv4) in H1.
+      rewrite H1 in *. simpl_format_list.
+      step_call parser_parse_udp_body; [ entailer | assumption | apply H2 ].
+    + apply is_sval_false_binary_op_eq in H1.
+      change (Val_eqb _ _) with (is_udp ipv4) in H1.
+      rewrite H1 in *. do 4 simpl_format_list. rewrite app_nil_r.
       step_call (@parser_accept_body Info). entailer.
 Qed.
 
@@ -137,8 +136,6 @@ Definition parser_parse_ethernet_spec: func_spec :=
     PATH p
     MOD (Some [["hdr"]]) [["packet_in"]]
     WITH (pin pin': packet_in) ether ipv4 hsample result
-         (_: ⊫ᵥ ethernet_repr_val ether \: ethernet_h)
-         (_: ⊫ᵥ ipv4_repr_val ipv4 \: ipv4_h)
          (_: if is_tcp ipv4 then ⊫ᵥ result \: tcp_h
              else if is_udp ipv4 then ⊫ᵥ result \: udp_h
                   else result = ValBaseNull)
@@ -146,7 +143,7 @@ Definition parser_parse_ethernet_spec: func_spec :=
                      ⦑ encode (ipv4_repr_val ipv4) ⦒;
                      ⦃ is_tcp ipv4 ? ⦑ encode result ⦒ |
                        ⦃ is_udp ipv4 ? ⦑ encode result ⦒ | ε ⦄ ⦄; ⦑ pin' ⦒] )
-         (_: ethernet_ether_type ether = P4BitV 16 ETHERTYPE_IPV4),
+         (_: P4BitV 16 (ethernet_ether_type ether) = P4BitV 16 ETHERTYPE_IPV4),
       PRE
         (ARG []
         (MEM [(["hdr"], (hdr hsample))]
@@ -162,9 +159,9 @@ Proof.
   start_function.
   simpl_format_list.
   step_call (@packet_in_extract_body Info);
-    [ entailer | apply extract_encode; [assumption | reflexivity] |].
-  step_if; change (ValBaseBit _) with (P4BitV 16 ETHERTYPE_IPV4) in H2;
-    rewrite abs_ether_eq_eq in H2.
+    [entailer | apply extract_encode; [apply ext_val_typ_ethernet | reflexivity] |].
+  step_if; change (ValBaseBit _) with (P4BitV 16 ETHERTYPE_IPV4) in H0;
+    rewrite abs_ether_eq_eq in H0.
   - unfold ethernet_extract_result.
     remember (Build_header_sample_rec
                 (header_sample_bridge hsample)
@@ -175,10 +172,9 @@ Proof.
                 (header_sample_udp hsample)) as new_hdr.
     assert (update "ethernet" (eval_val_to_sval (ethernet_repr_val ether))
               (hdr hsample) = hdr new_hdr) by (rewrite Heqnew_hdr; reflexivity).
-    rewrite H4.
-    step_call parser_parse_ipv4_body; [entailer | apply H0 | apply H1 | apply H5].
-  - apply is_sval_false_binary_op_eq in H2.
-    rewrite Val_eqb_neq_iff in H2. exfalso. apply H2. assumption.
+    rewrite H2. step_call parser_parse_ipv4_body; [entailer | apply H | apply H3].
+  - apply is_sval_false_binary_op_eq in H0.
+    rewrite Val_eqb_neq_iff in H0. exfalso. apply H0. assumption.
 Qed.
 
 Definition parser_parse_sample_fundef :=
@@ -196,8 +192,6 @@ Definition parser_parse_sample_spec: func_spec :=
     MOD (Some [["hdr"]]) [["packet_in"]]
     WITH (pin pin': packet_in) sample ether ipv4 hsample result
          (_: ⊫ᵥ sample \: sample_t)
-         (_: ⊫ᵥ ethernet_repr_val ether \: ethernet_h)
-         (_: ⊫ᵥ ipv4_repr_val ipv4 \: ipv4_h)
          (_: if is_tcp ipv4 then ⊫ᵥ result \: tcp_h
              else if is_udp ipv4 then ⊫ᵥ result \: udp_h
                   else result = ValBaseNull)
@@ -206,7 +200,7 @@ Definition parser_parse_sample_spec: func_spec :=
                      ⦑ encode (ipv4_repr_val ipv4) ⦒;
                      ⦃ is_tcp ipv4 ? ⦑ encode result ⦒ |
                        ⦃ is_udp ipv4 ? ⦑ encode result ⦒ | ε ⦄ ⦄; ⦑ pin' ⦒] )
-         (_: ethernet_ether_type ether = P4BitV 16 ETHERTYPE_IPV4),
+         (_: P4BitV 16 (ethernet_ether_type ether) = P4BitV 16 ETHERTYPE_IPV4),
       PRE
         (ARG []
         (MEM [(["hdr"], (hdr hsample))]
@@ -241,12 +235,16 @@ Qed.
 Definition parser_start_fundef :=
   ltac:(get_fd ["SwitchEgressParser"; "start"] ge).
 
-Definition bridge_repr_val (has_sample: Val): Val :=
-  ValBaseHeader [("contains_sample", has_sample)] true.
+Definition bridge_repr_val (has_sample: Z): Val :=
+  ValBaseHeader [("contains_sample", P4BitV 8 has_sample)] true.
 
-Definition contains_sample (has_sample: Val): bool := Val_eqb has_sample (P4BitV 8 1).
+Lemma ext_val_typ_bridge: forall has_sample, ⊫ᵥ bridge_repr_val has_sample \: bridge_t.
+Proof. intros. split; [repeat constructor | reflexivity]. Qed.
 
-Definition start_extract_result (has_sample: Val) (hsample : header_sample_rec)
+Definition contains_sample (has_sample: Z): bool :=
+  Val_eqb (P4BitV 8 has_sample) (P4BitV 8 1).
+
+Definition start_extract_result (has_sample: Z) (hsample : header_sample_rec)
   (sample : Val) (ether : ethernet_rec) (ipv4 : ipv4_rec) (result : Val) :=
   let bridge := eval_val_to_sval (bridge_repr_val has_sample) in
   let header := update "bridge" bridge (hdr hsample) in
@@ -261,11 +259,8 @@ Definition parser_start_spec: func_spec :=
     WITH (pin pin': packet_in) eg_intr_md has_sample sample
          hsample ether ipv4 result
          (_: ⊫ᵥ eg_intr_md \: egress_intrinsic_metadata_t)
-         (_: ⊫ᵥ bridge_repr_val has_sample \: bridge_t)
          (_: if contains_sample has_sample then ⊫ᵥ sample \: sample_t
              else sample = ValBaseNull)
-         (_: ⊫ᵥ ethernet_repr_val ether \: ethernet_h)
-         (_: ⊫ᵥ ipv4_repr_val ipv4 \: ipv4_h)
          (_: if is_tcp ipv4 then ⊫ᵥ result \: tcp_h
              else if is_udp ipv4 then ⊫ᵥ result \: udp_h
                   else result = ValBaseNull)
@@ -276,7 +271,7 @@ Definition parser_start_spec: func_spec :=
                      ⦑ encode (ipv4_repr_val ipv4) ⦒;
                      ⦃ is_tcp ipv4 ? ⦑ encode result ⦒ |
                        ⦃ is_udp ipv4 ? ⦑ encode result ⦒ | ε ⦄ ⦄; ⦑ pin' ⦒] )
-         (_: ethernet_ether_type ether = P4BitV 16 ETHERTYPE_IPV4),
+         (_: P4BitV 16 (ethernet_ether_type ether) = P4BitV 16 ETHERTYPE_IPV4),
       PRE
         (ARG []
         (MEM [(["hdr"], hdr hsample)]
@@ -306,13 +301,13 @@ Proof.
             ⦃ is_tcp ipv4 ? ⦑ encode result ⦒
             | ⦃ is_udp ipv4 ? ⦑ encode result ⦒ | ε ⦄ ⦄;
             ⦑ pin' ⦒].
-  change (⦑ encode eg_intr_md ⦒ :: l) with ([⦑ encode eg_intr_md ⦒] ++ l) in H5.
-  rewrite format_match_app_iff' in H5. destruct H5 as [p1 [p2 [? [? ?]]]].
-  step_call tofino_parser_body; [ entailer | eauto | apply H7 | ]. subst l.
+  change (⦑ encode eg_intr_md ⦒ :: l) with ([⦑ encode eg_intr_md ⦒] ++ l) in H2.
+  rewrite format_match_app_iff' in H2. destruct H2 as [p1 [p2 [? [? ?]]]].
+  step_call tofino_parser_body; [ entailer | eauto | apply H4 | ]. subst l.
   clear dependent pin. clear p1.
   simpl_format_list.
   step_call (@packet_in_extract_body Info);
-    [entailer | apply extract_encode; [assumption | reflexivity] | ].
+    [entailer | apply extract_encode; [ apply ext_val_typ_bridge | reflexivity] | ].
   remember (Build_header_sample_rec
               (eval_val_to_sval (bridge_repr_val has_sample))
               (header_sample_sample hsample)
@@ -321,17 +316,18 @@ Proof.
               (header_sample_tcp hsample)
               (header_sample_udp hsample)) as new_hdr.
   assert (Hu: update "bridge" (eval_val_to_sval (bridge_repr_val has_sample))
-            (hdr hsample) = hdr new_hdr) by (subst new_hdr; reflexivity).
-  rewrite Hu; step_if; rewrite Heqnew_hdr in H5; simpl in H5;
-    change (P4Bit 8 1) with (eval_val_to_sval (P4BitV 8 1)) in H5;
-    rewrite abs_eq_eq in H5.
-  - apply is_sval_true_binary_op_eq in H5.
-    change (Val_eqb _ _) with (contains_sample has_sample) in H5.
-    unfold start_extract_result. rewrite H5 in *. rewrite Hu. simpl_format_list.
+                (hdr hsample) = hdr new_hdr) by (subst new_hdr; reflexivity).
+  Opaque P4BitV.
+  rewrite Hu; step_if; rewrite Heqnew_hdr in H2; simpl in H2;
+    change (P4Bit 8 1) with (eval_val_to_sval (P4BitV 8 1)) in H2;
+    rewrite abs_eq_eq in H2. Transparent P4BitV.
+  - apply is_sval_true_binary_op_eq in H2.
+    change (Val_eqb _ _) with (contains_sample has_sample) in H2.
+    unfold start_extract_result. rewrite H2 in *. rewrite Hu. simpl_format_list.
     step_call parser_parse_sample_body; [entailer | eauto..].
-  - apply is_sval_false_binary_op_eq in H5.
-    change (Val_eqb _ _) with (contains_sample has_sample) in H5.
-    unfold start_extract_result. rewrite H5 in *. rewrite Hu.
+  - apply is_sval_false_binary_op_eq in H2.
+    change (Val_eqb _ _) with (contains_sample has_sample) in H2.
+    unfold start_extract_result. rewrite H2 in *. rewrite Hu.
     do 2 simpl_format_list.
     step_call parser_parse_ethernet_body; [entailer | eauto..].
 Qed.
@@ -345,11 +341,8 @@ Definition parser_spec: func_spec :=
     MOD (Some [["hdr"]; ["eg_md"]; ["eg_intr_md"]]) [["packet_in"]]
     WITH (pin pin': packet_in) eg_intr_md has_sample sample ether ipv4 result
          (_: ⊫ᵥ eg_intr_md \: egress_intrinsic_metadata_t)
-         (_: ⊫ᵥ bridge_repr_val has_sample \: bridge_t)
          (_: if contains_sample has_sample then ⊫ᵥ sample \: sample_t
              else sample = ValBaseNull)
-         (_: ⊫ᵥ ethernet_repr_val ether \: ethernet_h)
-         (_: ⊫ᵥ ipv4_repr_val ipv4 \: ipv4_h)
          (_: if is_tcp ipv4 then ⊫ᵥ result \: tcp_h
              else if is_udp ipv4 then ⊫ᵥ result \: udp_h
                   else result = ValBaseNull)
@@ -360,7 +353,7 @@ Definition parser_spec: func_spec :=
                      ⦑ encode (ipv4_repr_val ipv4) ⦒;
                      ⦃ is_tcp ipv4 ? ⦑ encode result ⦒ |
                        ⦃ is_udp ipv4 ? ⦑ encode result ⦒ | ε ⦄ ⦄; ⦑ pin' ⦒] )
-         (_: ethernet_ether_type ether = P4BitV 16 ETHERTYPE_IPV4),
+         (_: P4BitV 16 (ethernet_ether_type ether) = P4BitV 16 ETHERTYPE_IPV4),
       PRE
         (ARG []
         (MEM [(["hdr"], hdr hdr_init)]
